

1 Introduction: The Structure of Mathematical Reasoning

This document provides a structured overview of the core tools for formal reasoning in discrete mathematics: propositional logic, predicate logic, and standard proof techniques. The goal is to present a clear, procedural approach to constructing and analyzing mathematical arguments.

1.1 TOC

1	Introduction: The Structure of Mathematical Reasoning	1
1.1	TOC	1
2	Part I: Propositional Logic (Aussagenlogik)	1
2.1	Propositions and Connectives	1
2.2	Truth Tables and Logical Status	1
2.3	Logical Equivalences	1
3	Part II: Predicate Logic (Prädikatenlogik)	1
3.1	Predicates and Quantifiers	1
3.2	Nested Quantifiers	1
3.3	Negating Quantified Statements	1
3.4	Translating Natural Language	2
4	Part III: Proof Techniques (Beweismuster)	2
4.1	Direct Proof (Direkter Beweis)	2
4.2	Proof by Contraposition (Kontraposition)	2
4.3	Proof by Contradiction (Widerspruchsbeweis)	2
4.4	Proof by Cases (Fallunterscheidung)	2
4.5	Proof by Induction (Vollständige Induktion)	2

2 Part I: Propositional Logic (Aussagenlogik)

Propositional logic is the foundation of mathematical reasoning. It deals with propositions (statements that are either true or false) and the logical connectives that combine them.

2.1 Propositions and Connectives

Core Concepts

A **proposition** is a declarative sentence with a definite truth value (True/1 or False/0).

Connective	Symbol	Meaning
Negation	$\neg P$	“it is not the case that P
Conjunction	$P \wedge Q$	“P and Q are both true
Disjunction	$P \vee Q$	“at least one of P or Q is true
Implication	$P \rightarrow Q$	“if P is true, then Q is true
Biconditional	$P \leftrightarrow Q$	“P and Q have the same truth value

2.2 Truth Tables and Logical Status

Procedure: Constructing a Truth Table

- Create a column for each atomic proposition (n variables).
- Create 2^n rows to list all possible combinations of truth values.
- Add columns for complex sub-formulas, building up from simplest to most complex.

4. Fill each new column by applying the definition of its main connective to its constituent columns.

Example: Truth Table for $(P \vee Q) \rightarrow (P \wedge Q)$

P	Q	$P \vee Q$	$P \wedge Q$	$(P \vee Q) \rightarrow (P \wedge Q)$
0	0	0	0	1
0	1	1	0	0
1	0	1	0	0
1	1	1	1	1

Definitions of Logical Status

- Tautology:** A formula that is always true (final column is all 1s). E.g., $P \vee \neg P$.
- Contradiction:** A formula that is always false (final column is all 0s). E.g., $P \wedge \neg P$.
- Contingency:** A formula that is neither a tautology nor a contradiction.
- Satisfiable:** A formula that is true for at least one assignment of truth values (i.e., not a contradiction).

2.3 Logical Equivalences

Concept

Two formulas F and G are **logically equivalent** ($F \equiv G$) if they have identical truth tables. This means $F \equiv G$ is a tautology. Equivalences are the rules for algebraic manipulation of logical formulas.

Fundamental Laws

- De Morgan’s Laws:** $\neg(P \wedge Q) \equiv (\neg P \vee \neg Q)$ $\neg(P \vee Q) \equiv (\neg P \wedge \neg Q)$
- Distributive Laws:** $P \wedge (Q \vee R) \equiv (P \wedge Q) \vee (P \wedge R)$ $P \vee (Q \wedge R) \equiv (P \vee Q) \wedge (P \vee R)$
- Implication Equivalence:** $P \rightarrow Q \equiv \neg P \vee Q$
- Contrapositive:** $P \rightarrow Q \equiv \neg Q \rightarrow \neg P$
- Biconditional Equivalence:** $P \equiv Q \equiv (P \rightarrow Q) \wedge (Q \rightarrow P)$
- Double Negation:** $\neg(\neg P) \equiv P$

TA Tip: The Implication Pitfall

The expression $P \rightarrow Q$ is only false when a true premise leads to a false conclusion ($T \rightarrow F$). If the premise P is false, the implication is **vacuously true**. This is a common source of confusion but is essential for mathematical reasoning.

3 Part II: Predicate Logic (Prädikatenlogik)

Predicate logic extends propositional logic by introducing variables, predicates, and quantifiers, allowing for statements about properties of objects and relationships between them.

3.1 Predicates and Quantifiers

- Universe of Discourse (\mathbb{U}):** The non-empty set of objects that variables can represent (e.g., integers, people, all cats).

- Predicate:** A property that becomes a proposition when its variables are assigned values from the UoD. E.g., $P(x) = x > 3$.
- Universal Quantifier (\forall):** “For all”. $\forall x, P(x)$ is true if $P(x)$ is true for every x in the UoD.
- Existential Quantifier (\exists):** “There exists”. $\exists x, P(x)$ is true if there is at least one x in the UoD for which $P(x)$ is true.

3.2 Nested Quantifiers

Procedure for Interpretation

- Read from left to right. The order is critical.
- The choice for a variable bound by an inner quantifier can depend on the variables of the outer quantifiers.
- Think of it as a nested loop or a challenge-response game: $\forall x$ means “for any x an opponent gives you...”, $\exists y$ means “...you can find a y such that...”.

Simple Example

UoD = Integers.

- $\forall x \exists y, x < y$: “For every integer, there is a larger integer.” (True, choose $y = x + 1$).
- $\exists y \forall x, x < y$: “There exists an integer that is larger than all integers.” (False, no maximum integer exists).

Harder Example

UoD = People. $L(x, y) = x$ loves y .

- $\forall x \exists y, L(x, y)$: “Everybody loves somebody.” (The person loved can be different for each individual).
- $\exists y \forall x, L(x, y)$: “There is somebody who is loved by everybody.” (A single, universally loved person exists).

3.3 Negating Quantified Statements

Procedure (De Morgan’s for Quantifiers)

- Place a \neg in front of the entire quantified statement.
- “Push” the \neg inward across each quantifier one by one.
- Each time the \neg passes a quantifier, the quantifier flips (\forall becomes \exists , and vice versa).
- Once inside, apply standard propositional De Morgan’s laws to the predicate expression.

Simple Example

$\neg(\forall x P(x)) \equiv \exists x \neg P(x)$

$\neg(\exists x P(x)) \equiv \forall x \neg P(x)$

Harder Example

Statement: “All students who studied passed the exam.” $\forall x((S(x) \wedge T(x)) \rightarrow P(x))$

Negation Procedure:

- $\neg(\forall x((S(x) \wedge T(x)) \rightarrow P(x)))$
- $\equiv \exists x \neg((S(x) \wedge T(x)) \rightarrow P(x))$ (Flip \forall , push \neg in)
- $\equiv \exists x \neg(\neg(S(x) \wedge T(x)) \vee P(x))$ (Implication law)
- $\equiv \exists x(S(x) \wedge T(x)) \wedge \neg P(x)$ (De Morgan’s & Double Negation)

Meaning: “There exists someone who is a student, studied, and did not pass.”

3.4 Translating Natural Language

Procedure for Translation

1. Define the Universe of Discourse (\mathbb{U}).
2. Define predicates for each property (e.g., $C(x)$ for “ x is a cat”).
3. Identify the main logical structure ($\forall, \exists, \rightarrow, \neg, \wedge$).
4. Translate piece by piece, adhering to the standard patterns.

Standard Patterns

- “All A’s are B’s”: $\forall x(A(x) \rightarrow B(x))$
- “Some A’s are B’s”: $\exists x(A(x) \wedge B(x))$
- “No A’s are B’s”: $\forall x(A(x) \rightarrow \neg B(x))$
- “Not all A’s are B’s”: $\exists x(A(x) \wedge \neg B(x))$

The Golden Rule of Translation:

- Use \rightarrow as the main connective with \forall .
- Use \wedge as the main connective with \exists .

Why?

- $\forall x(A(x) \wedge B(x))$ means “Everything in the universe is both an A and a B”. This is almost always too strong.
- $\exists x(A(x) \rightarrow B(x))$ means “There exists something that, if it’s an A, is also a B”. This is true if there’s just one thing in the UoD that is **not** an A, making it too weak and usually not what is intended.

4 Part III: Proof Techniques (Beweismuster)

This section outlines the fundamental strategies for constructing mathematical proofs. A systematic approach involves identifying the claim’s structure and selecting the most appropriate technique.

4.1 Direct Proof (Direkter Beweis)

Procedure

To prove an implication $P \rightarrow Q$:

1. Assume P is true.
2. Use definitions, axioms, and established theorems to build a logical chain of deductions.
3. Conclude that Q must be true.

Simple Example

Claim: If n is an odd integer, then n^2 is odd.

Proof: Assume n is odd. By definition, $n = 2k + 1$ for some integer k . Then $n^2 = (2k + 1)^2 = 4k^2 + 4k + 1 = 2(2k^2 + 2k) + 1$. Let $m = 2k^2 + 2k$. Since k is an integer, m is an integer. Thus, $n^2 = 2m + 1$, which is the definition of an odd number.

4.2 Proof by Contraposition (Kontraposition)

Procedure

To prove $P \rightarrow Q$, instead prove its logically equivalent contrapositive, $\neg Q \rightarrow \neg P$. This is often simpler when the conclusion Q is a negative statement.

1. Assume $\neg Q$ is true.
2. Follow logical steps to show that $\neg P$ must be true.

Simple Example

Claim: For an integer n , if n^2 is even, then n is even.

Proof: The contrapositive is “If n is not even (odd), then n^2 is not even (odd).” This is precisely the statement proven in the Direct Proof example above. Since the contrapositive is true, the original statement is true.

4.3 Proof by Contradiction (Widerspruchsbeweis)

Procedure

To prove a statement P :

1. Assume $\neg P$ is true.
2. From this assumption, derive a logical contradiction (a statement of the form $R \wedge \neg R$).
3. Conclude that the assumption $\neg P$ must be false, hence P is true.

Harder Example: Infinitude of Primes

Claim: There are infinitely many prime numbers.

Proof:

1. Assume for contradiction that there is a finite number of primes. Let them be p_1, p_2, \dots, p_n .
2. Consider the number $N = (p_1 \times p_2 \times \dots \times p_n) + 1$.
3. N must have a prime factor. Let this prime factor be p .
4. This prime p must be one of the primes in our list, so $p = p_i$ for some i .
5. This means p_i divides N . But p_i also divides the product $p_1 \times \dots \times p_n$.
6. If p_i divides both numbers, it must divide their difference: $N - (p_1 \times \dots \times p_n) = 1$.
7. **Contradiction:** No prime number can divide 1.
8. Therefore, the assumption of a finite number of primes is false.

4.4 Proof by Cases (Fallunterscheidung)

Procedure

1. Partition the problem domain into a set of exhaustive cases C_1, C_2, \dots, C_k .
2. Prove the statement for each case individually.
3. Since the cases cover all possibilities, the statement holds universally.

Simple Example

Claim: For any integer n , $n^2 \geq n$.

Proof:

- **Case 1:** $n \geq 1$. Multiplying both sides of $n \geq 1$ by the positive number n gives $n^2 \geq n$.
- **Case 2:** $n = 0$. $0^2 \geq 0$ becomes $0 \geq 0$, which is true.
- **Case 3:** $n < 0$. Here, n^2 is non-negative, while n is negative. Any non-negative number is greater than any negative number, so $n^2 > n$.

Since the statement holds in all three exhaustive cases, it is true for all integers.

4.5 Proof by Induction (Vollständige Induktion)

Procedure (Weak Induction)

To prove $\forall n \geq n_0, P(n)$:

1. **Base Case (Induktionsanfang):** Verify $P(n_0)$ is true.

2. **Inductive Hypothesis (Annahme):** Assume $P(k)$ is true for an arbitrary $k \geq n_0$.
3. **Inductive Step (Schritt):** Using the hypothesis, prove that $P(k + 1)$ is also true.

Simple Example (Weak)

Claim: $\sum_{i=1}^n i = \frac{n(n+1)}{2}$ for $n \geq 1$.

Proof:

- **Base Case (n=1):** $\sum_{i=1}^1 i = 1$. And $1 \frac{1+1}{2} = 1$. True.
- **Hypothesis:** Assume $\sum_{i=1}^k i = \frac{k(k+1)}{2}$.
- **Step:** Show for $k + 1$: $\sum_{i=1}^{k+1} i = \left(\sum_{i=1}^k i \right) + (k + 1)$
$$= \frac{k(k+1)}{2} + (k + 1)$$

(by hypothesis) $= (k + 1) \left(\frac{k}{2} + 1 \right) = (k + 1) \frac{k+2}{2}$. This is the required formula for $n = k + 1$.

Procedure (Strong Induction)

Strong induction assumes truth for all prior cases up to k , while weak assumes only for k .

1. **Base Case(s):** Verify $P(n_0)$ (and possibly more initial cases).
2. **Hypothesis:** Assume $P(j)$ is true for **all** integers j where $n_0 \leq j \leq k$.
3. **Step:** Using the hypothesis, prove $P(k + 1)$ is true.

Harder Example (Strong)

Claim: Any postage of $n \geq 12$ cents can be made with 4- and 5-cent stamps.

Proof:

- **Base Cases:** $P(12) : 3 \times 4$. True. $P(13) : 2 \times 4 + 1 \times 5$. True. $P(14) : 1 \times 4 + 2 \times 5$. True. $P(15) : 3 \times 5$. True.
- **Hypothesis:** Assume for an arbitrary $k \geq 15$, $P(j)$ is true for all j with $12 \leq j \leq k$.
- **Step:** We want to show $P(k + 1)$. Consider the postage for $k - 3$. Since $k \geq 15$, $k - 3 \geq 12$. By our strong hypothesis, we know we can make postage for $k - 3$. To get postage for $k + 1$, we simply add a 4-cent stamp: $(k - 3) + 4 = k + 1$. Thus, $P(k + 1)$ is true.